
\documentclass[12pt,a4paper,draft]{article}
\newcommand\tab[1][1cm]{\hspace*{#1}}
\usepackage[utf8]{inputenc}
%\usepackage[russian]{babel}
\usepackage[OT1]{fontenc}
\usepackage{cmap}
\usepackage{amsmath}
\usepackage{amsfonts}
\usepackage{amssymb}
%\usepackage{txfonts}
%\usepackage{mathptmx}
\usepackage{setspace}
\usepackage[left=2cm,right=2cm,top=2cm,bottom=2cm]{geometry}
\usepackage{graphicx}
\DeclareGraphicsExtensions{.pdf,.png,.jpg}
\graphicspath{{imgs/}}
\linespread{1.5}
\onehalfspacing
\begin{document}
Target equation:
\\$
-i a_{1} u^{(1,0)}(x,t)+a_{2} u^{(2,0)}(x,t)-i a_{3} u^{(3,0)}(x,t)+a_{4} u^{(4,0)}(x,t)-i a_{5} u^{(5,0)}(x,t)+a_{6} u^{(6,0)}(x,t)-b u(x,t) \left| u(x,t)\right| ^2+i u^{(0,1)}(x,t)=0
$\\
Substitutions:
$$
\begin{array}{c}
 \text{N = 3} \\
 u(x,t)\to y(z) e^{i (k x-\omega  t)} \\
 z\to x-\text{C0} t \\
 y(z)\to A R(z)^3 \\
 R'(z)^2=R(z)^2 \left(1-\chi  R(z)^2\right) \\
\end{array}
$$
Imaginary part of equation after substitutions:
\\$
y'(z) \left(a_{1}-2 a_{2} k-3 a_{3} k^2+4 a_{4} k^3+5 a_{5} k^4-6 a_{6} k^5-\text{C0}\right)+y^{(3)}(z) \left(a_{3}-4 a_{4} k-10 a_{5} k^2+20 a_{6} k^3\right)+y^{(5)}(z) (a_{5}-6 a_{6} k)=0
$\\
Real part of equation after substitutions:
\\$
y(z) \left(a_{1} k-a_{2} k^2-a_{3} k^3+a_{4} k^4+a_{5} k^5-a_{6} k^6+\omega \right)+y''(z) \left(a_{2}+3 a_{3} k-6 a_{4} k^2-10 a_{5} k^3+15 a_{6} k^4\right)+a_{4} y^{(4)}(z)+5 a_{5} k y^{(4)}(z)-15 a_{6} k^2 y^{(4)}(z)+a_{6} y^{(6)}(z)-b y(z)^3=0
$\\
Constraints on coefficients from imaginary part of equation:
\\$a_{5}\to 6 a_{6} k$\\
$a_{3}\to 4 \left(a_{4} k+10 a_{6} k^3\right)$\\
$\text{C0}\to a_{1}-2 a_{2} k-8 a_{4} k^3-96 a_{6} k^5$\\
Constraints on coefficients from real part of equation:
\\$b\to -\frac{20160 a_{6} \chi ^3}{A^2}$\\
$a_{4}\to -a_{6} \left(15 k^2+83\right)$\\
$a_{2}\to 15 a_{6} k^4+498 a_{6} k^2+1891 a_{6}$\\
$\omega \to -a_{1} k+5 a_{6} k^6+249 a_{6} k^4+1891 a_{6} k^2-11025 a_{6}$\\


y(z) - function:
$$
\frac{64 a^3 A}{\left(4 a^2 e^z+\chi  e^{-z}\right)^3}
$$
u(x, t) - function:
$$
\frac{64 a^3 A e^{i (k x-\omega  t)}}{\left(4 a^2 e^{\text{C0} t+x}+\chi  e^{-\text{C0} t-x}\right)^3}
$$

\end{document}
