
\documentclass[12pt,a4paper,draft]{article}
\newcommand\tab[1][1cm]{\hspace*{#1}}
\usepackage[utf8]{inputenc}
%\usepackage[russian]{babel}
\usepackage[OT1]{fontenc}
\usepackage{cmap}
\usepackage{amsmath}
\usepackage{amsfonts}
\usepackage{amssymb}
%\usepackage{txfonts}
%\usepackage{mathptmx}
\usepackage{setspace}
\usepackage[left=2cm,right=2cm,top=2cm,bottom=2cm]{geometry}
\usepackage{graphicx}
\DeclareGraphicsExtensions{.pdf,.png,.jpg}
\graphicspath{{imgs/}}
\linespread{1.5}
\onehalfspacing
\begin{document}
Target equation:
$$
-i \text{a1} u^{(1,0)}(x,t)+\text{a2} u^{(2,0)}(x,t)-i \text{a3} u^{(3,0)}(x,t)+\text{a4} u^{(4,0)}(x,t)-b u(x,t) \left| u(x,t)\right| ^2+i u^{(0,1)}(x,t)=0
$$
Substitutions:
$$
\begin{array}{c}
 \text{N = 2} \\
 u(x,t)\to y(z) e^{i (k x-\omega  t)} \\
 z\to x-\text{C0} t \\
 y(z)\to A R(z)^2 \\
 R'(z)^2=R(z)^2 \left(1-\chi  R(z)^2\right) \\
\end{array}
$$
Imaginary part of equation after substitutions:
$$
y'(z) \left(\text{a1}-2 \text{a2} k-3 \text{a3} k^2+4 \text{a4} k^3-\text{C0}\right)+y^{(3)}(z) (\text{a3}-4 \text{a4} k)=0
$$
Real part of equation after substitutions:
$$
y(z) \left(\text{a1} k-\text{a2} k^2-\text{a3} k^3+\text{a4} k^4+\omega \right)+y''(z) (\text{a2}+3 k (\text{a3}-2 \text{a4} k))+\text{a4} y^{(4)}(z)-b y(z)^3=0
$$
Constraints on coefficients from imaginary part of equation:
$$
\begin{array}{c}
 \text{a3}\to 4 \text{a4} k \\
 \text{C0}\to \text{a1}-2 \text{a2} k-8 \text{a4} k^3 \\
\end{array}
$$
Constraints on coefficients from real part of equation:
$$
\begin{array}{c}
 b\to \frac{120 \text{a4} \chi ^2}{A^2} \\
 \text{a2}\to -2 \left(3 \text{a4} k^2+10 \text{a4}\right) \\
 \omega \to -\text{a1} k-3 \text{a4} k^4-20 \text{a4} k^2+64 \text{a4} \\
\end{array}
$$


y(z) - function:
$$
\frac{16 a^2 A}{\left(4 a^2 e^z+\chi  e^{-z}\right)^2}
$$
u(x, t) - function:
$$
\frac{16 a^2 A e^{i (k x-\omega  t)}}{\left(4 a^2 e^{\text{C0} t+x}+\chi  e^{-\text{C0} t-x}\right)^2}
$$

\end{document}